The invariant about RqDown/RsDown message orders

src/RqRsInvLock.v
@@ -12,18 +12,20 @@ Open Scope list.
 Open Scope fmap.
 
 Ltac good_locking_get obj :=
-  match goal with
-  | [Hlock: UpLockInv _ ?sys _, Ho: In obj (sys_objs ?sys) |- _] =>
-    let H := fresh "H" in
-    pose proof Hlock as H;
-    specialize (H (obj_idx obj)); simpl in H;
-    specialize (H (in_map _ _ _ Ho)); dest
-  | [Hlock: DownLockInv _ ?sys _, Ho: In obj (sys_objs ?sys) |- _] =>
-    let H := fresh "H" in
-    pose proof Hlock as H;
-    specialize (H (obj_idx obj)); simpl in H;
-    specialize (H (in_map _ _ _ Ho)); dest
-  end.
+  try match goal with
+      | [Hlock: UpLockInv _ ?sys _, Ho: In obj (sys_objs ?sys) |- _] =>
+        let H := fresh "H" in
+        pose proof Hlock as H;
+        specialize (H (obj_idx obj)); simpl in H;
+        specialize (H (in_map _ _ _ Ho)); dest
+      end;
+  try match goal with
+      | [Hlock: DownLockInv _ ?sys _, Ho: In obj (sys_objs ?sys) |- _] =>
+        let H := fresh "H" in
+        pose proof Hlock as H;
+        specialize (H (obj_idx obj)); simpl in H;
+        specialize (H (in_map _ _ _ Ho)); dest
+      end.
 
 Ltac disc_lock_conds :=
   match goal with
@@ -36,5 +38,521 @@ Ltac disc_lock_conds :=
     destruct H as [rqUp [down [pidx ?]]]; dest
   end.
 
+Section RqRsDown.
+  Context {oifc: OStateIfc}.
+  Variables (dtr: DTree)
+            (sys: System oifc).
+  Hypothesis (Hrrs: RqRsSys dtr sys).
+
+  Definition ONoDownLock (orqs: ORqs Msg) (oidx: IdxT) :=
+    orqs@[oidx] >>=[True] (fun orq => orq@[downRq] = None).
+
+  Definition ODownRq (orqs: ORqs Msg) (msgs: MessagePool Msg) (oidx: IdxT) (down: IdxT) :=
+    orqs@[oidx] >>=[False]
+        (fun orq =>
+           orq@[downRq] >>=[False]
+              (fun rqid =>
+                 forall cidx rsUp,
+                   edgeDownTo dtr cidx = Some down ->
+                   rsEdgeUpFrom dtr cidx = Some rsUp ->
+                   In rsUp rqid.(rqi_minds_rss) ->
+                   rqsQ msgs down <> nil)).
+  
+  Definition NoRqRsDown (st: MState oifc) :=
+    forall cobj pobj,
+      In cobj sys.(sys_objs) ->
+      In pobj sys.(sys_objs) ->
+      parentIdxOf dtr (obj_idx cobj) = Some (obj_idx pobj) ->
+      forall down,
+        edgeDownTo dtr (obj_idx cobj) = Some down ->
+        forall rsdm,
+          rsdm.(msg_type) = MRs ->
+          InMP down rsdm st.(bst_msgs) ->
+          ONoDownLock st.(bst_orqs) (obj_idx pobj) \/
+          (ODownRq st.(bst_orqs) st.(bst_msgs) (obj_idx pobj) down /\
+           FirstMP st.(bst_msgs) down rsdm).
+  
+  Lemma noRqRsDown_InvInit:
+    InvInit sys NoRqRsDown.
+  Proof.
+    do 2 red; intros.
+    simpl in *.
+    inv H4.
+  Qed.
+
+  Lemma noRqRsDown_step_ext_in:
+    forall oss orqs msgs eins,
+      NoRqRsDown {| bst_oss := oss; bst_orqs := orqs; bst_msgs := msgs |} ->
+      eins <> nil ->
+      ValidMsgsExtIn sys eins ->
+      NoRqRsDown {| bst_oss := oss;
+                    bst_orqs := orqs;
+                    bst_msgs := enqMsgs eins msgs |}.
+  Proof.
+  Admitted.
+
+  Lemma noRqRsDown_step_ext_out:
+    forall oss orqs msgs eouts,
+      NoRqRsDown {| bst_oss := oss; bst_orqs := orqs; bst_msgs := msgs |} ->
+      eouts <> nil ->
+      Forall (FirstMPI msgs) eouts ->
+      ValidMsgsExtOut sys eouts ->
+      NoRqRsDown {| bst_oss := oss;
+                    bst_orqs := orqs;
+                    bst_msgs := deqMsgs (idsOf eouts) msgs |}.
+  Proof.
+  Admitted.
+
+  Ltac disc_NoRqRsDown :=
+    match goal with
+    | [H: NoRqRsDown _ |- NoRqRsDown _] =>
+      let cobj := fresh "cobj" in
+      let pobj := fresh "pobj" in
+      let H0 := fresh in
+      let H1 := fresh in
+      let H2 := fresh in
+      let down := fresh "down" in
+      let H3 := fresh in
+      let rsdm := fresh "rsdm" in
+      let H4 := fresh in
+      red; intros cobj pobj H0 H1 H2 down H3 rsdm H4 ?;
+      specialize (H _ _ H0 H1 H2 _ H3 _ H4); simpl in *
+    end.
+  
+  Ltac disc_rule_custom ::=
+    try disc_footprints_ok;
+    try disc_NoRqRsDown.
+
+  Lemma noRqRsDown_step_int:
+    forall st1,
+      Reachable (steps step_m) sys st1 ->
+      NoRqRsDown st1 ->
+      forall oidx ridx rins routs st2,
+        step_m sys st1 (RlblInt oidx ridx rins routs) st2 ->
+        NoRqRsDown st2.
+  Proof.
+    destruct Hrrs as [? [? ?]]; intros.
+    pose proof (footprints_ok H0 H2) as Hftinv.
+    assert (Reachable (steps step_m) sys st2) as Hnrch
+      by (eapply reachable_steps; [eassumption|apply steps_singleton; eassumption]).
+    pose proof (upLockInv_ok H0 H Hnrch) as Hulinv.
+    pose proof (downLockInv_ok H0 H H2) as Hdlinv.
+    clear Hnrch.
+
+    inv_step.
+    good_rqrs_rule_get rule.
+    good_rqrs_rule_cases rule.
+
+    - disc_rule_conds.
+      destruct (eq_nat_dec (obj_idx obj) (obj_idx pobj)).
+      + eapply obj_same_id_in_system_same in e; eauto; subst.
+        left; red; mred.
+      + apply InMP_enqMP_or in H11; destruct H11;
+          [exfalso; dest; subst; disc_rule_conds; auto|].
+        apply InMP_deqMP in H11.
+        specialize (H3 H11); destruct H3.
+        * left; red; mred.
+        * dest; right; split.
+          { red in H3; red; mred.
+            destruct (orqs@[obj_idx pobj]) eqn:Horq; simpl in *; auto.
+            destruct (o@[downRq]) eqn:Hrqid; simpl in *; auto.
+            intros; specialize (H3 _ _ H20 H23 H27).
+            assert (cidx <> cidx0) by (intro Hx; subst; disc_rule_conds; auto).
+            solve_q; assumption.
+          }
+          { apply FirstMP_enqMP.
+            apply FirstMP_deqMP; [|assumption].
+            solve_midx_neq.
+          }
+
+    - disc_rule_conds.
+      destruct (eq_nat_dec (obj_idx obj) (obj_idx pobj)).
+      + eapply obj_same_id_in_system_same in e; eauto; subst.
+        left; red; mred.
+      + apply InMP_enqMP_or in H18; destruct H18;
+          [exfalso; dest; subst; solve_midx_false|].
+        apply InMP_deqMP in H14; specialize (H3 H14).
+        destruct (eq_nat_dec (obj_idx cobj) (obj_idx obj)).
+        * exfalso.
+          eapply obj_same_id_in_system_same in e; eauto; subst.
+          disc_rule_conds.
+          destruct H3.
+          { good_locking_get pobj.
+            eapply downLockInvORq_down_rqsQ_length_one_locked in H6; eauto;
+              [|eapply rqsQ_length_ge_one; eauto;
+                apply FirstMP_InMP; auto].
+            destruct H6 as [rqid ?]; dest.
+            red in H3.
+            destruct (orqs@[obj_idx pobj]) as [orq|]; simpl in *; [|discriminate].
+            congruence.
+          }
+          { dest; pose proof (FirstMP_eq H7 H24).
+            subst; simpl in *.
+            rewrite H8 in H27; discriminate.
+          }
+        * destruct H3; [left; red; mred|].
+          dest; right; split.
+          { red in H3; red; mred.
+            destruct (orqs@[obj_idx pobj]) eqn:Horq; simpl in *; auto.
+            destruct (o@[downRq]) eqn:Hrqid; simpl in *; auto.
+            intros; specialize (H3 _ _ H20 H22 H26).
+            solve_q; assumption.
+          }
+          { apply FirstMP_enqMP.
+            apply FirstMP_deqMP; [|assumption].
+            solve_midx_neq.
+          }
+
+    - disc_rule_conds.
+      + apply InMP_enqMP_or in H31; destruct H31;
+          [exfalso; dest; subst; disc_rule_conds; auto|].
+        apply InMP_deqMP in H14.
+        specialize (H3 H14).
+        destruct (eq_nat_dec (obj_idx obj) (obj_idx pobj)).
+        * eapply obj_same_id_in_system_same in e; eauto; subst.
+          destruct H3.
+          { left; red in H3; red; repeat (simpl; mred). }
+          { dest; right; split.
+            { red in H3; red; repeat (simpl; mred).
+              destruct (porq@[downRq]) eqn:Hrqid; simpl in *; auto.
+              intros; specialize (H3 _ _ H26 H31 H34).
+              solve_q; assumption.
+            }
+            { apply FirstMP_enqMP.
+              apply FirstMP_deqMP; [|assumption].
+              solve_midx_neq.
+            }
+          }
+        * destruct H3.
+          { left; red in H3; red; mred. }
+          { dest; right; split.
+            { red in H3; red; mred.
+              destruct (orqs@[obj_idx pobj]) eqn:Horq; simpl in *; auto.
+              destruct (o@[downRq]) eqn:Hrqid; simpl in *; auto.
+              intros; specialize (H3 _ _ H26 H31 H34).
+              solve_q; assumption.
+            }
+            { apply FirstMP_enqMP.
+              apply FirstMP_deqMP; [|assumption].
+              solve_midx_neq.
+            }
+          }
+
+      + apply InMP_enqMsgs_or in H33; destruct H33.
+        1:{ exfalso.
+            rewrite Forall_forall in H32; specialize (H32 _ H5).
+            simpl in H32; rewrite H31 in H32; discriminate.
+        }
+        apply InMP_deqMP in H5.
+        specialize (H3 H5).
+        destruct (eq_nat_dec (obj_idx obj) (obj_idx pobj)).
+        * eapply obj_same_id_in_system_same in e; eauto; subst.
+          destruct H3; [|dest; exfalso; red in H3; mred].
+          right; split.
+          { destruct (in_dec eq_nat_dec down (idsOf routs)).
+            { red; repeat (simpl; mred).
+              intros; solve_q.
+              destruct H19.
+              apply in_map_iff in i; destruct i as [[down' rqdm] ?]; dest.
+              simpl in *; subst.
+              erewrite findQ_In_NoDup_enqMsgs; try eassumption.
+              rewrite Forall_forall in H32; specialize (H32 _ H36); simpl in H32.
+              rewrite filter_app; simpl.
+              rewrite H32; simpl.
+              destruct (filter _ _); discriminate.
+            }
+            { red; repeat (simpl; mred).
+              intros; disc_rule_conds.
+              elim n; clear n.
+              eapply RqRsDownMatch_rs_rq in H20; [|eassumption].
+              destruct H20 as [cidx [rdown ?]]; dest.
+              disc_rule_conds.
+            }
+          }
+          { apply FirstMP_enqMsgs.
+            apply FirstMP_deqMP.
+            { solve_midx_neq. }
+            { (* [rqsQ down msgs = nil] since [porq@[downRq] = None].
+               * Need to prove:
+               * [InMP down rsdm msgs -> rqsQ down msgs = nil -> FirstMP down rsdm msgs]
+               *)
+              admit.
+            }
+          }
+        * destruct H3; [left; red; mred|].
+          dest; right; split.
+          { red in H3; red; mred.
+            destruct (orqs@[obj_idx pobj]) eqn:Horq; simpl in *; auto.
+            destruct (o@[downRq]) eqn:Hrqid; simpl in *; auto.
+            intros; specialize (H3 _ _ H24 H33 H34).
+            disc_rule_conds.
+            assert (Some (obj_idx pobj) <> Some (obj_idx obj)) by congruence.
+            solve_q; assumption.
+          }
+          { apply FirstMP_enqMsgs.
+            apply FirstMP_deqMP; [|assumption].
+            solve_midx_neq.
+          }
+
+      + apply InMP_enqMsgs_or in H27; destruct H27.
+        1:{ exfalso.
+            rewrite Forall_forall in H32; specialize (H32 _ H14).
+            simpl in H32; rewrite H25 in H32; discriminate.
+        }
+        apply InMP_deqMP in H14.
+        specialize (H3 H14).
+        destruct (eq_nat_dec (obj_idx obj) (obj_idx pobj)).
+        * eapply obj_same_id_in_system_same in e; eauto; subst.
+          right; split.
+          { destruct (in_dec eq_nat_dec down (idsOf routs)).
+            { red; repeat (simpl; mred).
+              intros; solve_q.
+              destruct H19.
+              apply in_map_iff in i; destruct i as [[down' rqdm] ?]; dest.
+              simpl in *; subst.
+              erewrite findQ_In_NoDup_enqMsgs; try eassumption.
+              rewrite Forall_forall in H32; specialize (H32 _ H34); simpl in H32.
+              rewrite filter_app; simpl.
+              rewrite H32; simpl.
+              destruct (filter _ _); discriminate.
+            }
+            { red; repeat (simpl; mred).
+              intros; disc_rule_conds.
+              elim n; clear n.
+              eapply RqRsDownMatch_rs_rq in H6; [|eassumption].
+              destruct H6 as [cidx [rdown ?]]; dest.
+              disc_rule_conds.
+            }
+          }
+          { apply FirstMP_enqMsgs.
+            apply FirstMP_deqMP.
+            { apply parentIdxOf_not_eq in H20; [|apply Hrrs].
+              solve_midx_neq.
+            }
+            { (* Need to prove:
+               * [InMP down rsdm msgs -> rqsQ down msgs = nil -> FirstMP down rsdm msgs]
+               *)
+              admit.
+            }
+          }
+          
+        * destruct (eq_nat_dec (obj_idx obj) (obj_idx cobj)).
+          { eapply obj_same_id_in_system_same in e; eauto; subst.
+            disc_rule_conds.
+            exfalso; destruct H3.
+            { good_locking_get pobj.
+              eapply downLockInvORq_down_rqsQ_length_one_locked in H20; eauto;
+                [|eapply rqsQ_length_ge_one; eauto;
+                  apply FirstMP_InMP; auto].
+              destruct H20 as [rqid ?]; dest.
+              red in H3.
+              destruct (orqs@[obj_idx pobj]) as [orq|]; simpl in *; [|discriminate].
+              congruence.
+            }
+            { dest; pose proof (FirstMP_eq H23 H29).
+              subst; simpl in *.
+              rewrite H25 in H30; discriminate.
+            }
+          }
+          { destruct H3; [left; red; mred|].
+            dest; right; split.
+            { red in H3; red; mred.
+              destruct (orqs@[obj_idx pobj]) eqn:Horq; simpl in *; auto.
+              destruct (o@[downRq]) eqn:Hrqid; simpl in *; auto.
+              intros; specialize (H3 _ _ H26 H27 H31).
+              disc_rule_conds.
+              assert (Some (obj_idx pobj) <> Some (obj_idx obj)) by congruence.
+              solve_q; assumption.
+            }
+            { apply FirstMP_enqMsgs.
+              apply FirstMP_deqMP; [|assumption].
+              solve_midx_neq.
+            }
+          }
+
+    - good_footprint_get (obj_idx obj).
+      disc_rule_conds.
+      + apply InMP_enqMP_or in H26; destruct H26.
+        * dest; subst; disc_rule_conds.
+          eapply obj_same_id_in_system_same in H26; eauto; subst.
+          left; red; repeat (simpl; mred).
+        * destruct (eq_nat_dec (obj_idx obj) (obj_idx pobj)).
+          { apply InMP_deqMP in H26.
+            specialize (H3 H26).
+            eapply obj_same_id_in_system_same in e; eauto; subst.
+            destruct H3.
+            { left; red in H3; red; repeat (simpl; mred). }
+            { dest; right; split.
+              { red in H3; red; mred. }
+              { apply FirstMP_enqMP.
+                apply FirstMP_deqMP; [|assumption].
+                apply parentIdxOf_not_eq in H18; [|apply Hrrs].
+                solve_midx_neq.
+              }
+            }
+          }
+          { destruct (eq_nat_dec (obj_idx obj) (obj_idx cobj)).
+            { exfalso.
+              eapply obj_same_id_in_system_same in e; eauto; subst.
+              disc_rule_conds.
+              (* H26 is false. *)
+              admit.
+            }
+            { apply InMP_deqMP in H26; specialize (H3 H26).
+              destruct H3; [left; red in H3; red; mred|].
+              dest; right; split.
+              { red in H3; red; mred.
+                destruct (orqs@[obj_idx pobj]) eqn:Horq; simpl in *; auto.
+                destruct (o@[downRq]) eqn:Hrqid; simpl in *; auto.
+                intros; specialize (H3 _ _ H32 H33 H34).
+                disc_rule_conds.
+                assert (cidx <> obj_idx cobj)
+                  by (intro Hx; subst; disc_rule_conds; auto).
+                solve_q; assumption.
+              }
+              { apply FirstMP_enqMP.
+                apply FirstMP_deqMP; [|assumption].
+                solve_midx_neq.
+              }
+            }
+          }
+
+      + apply InMP_enqMP_or in H27; destruct H27.
+        * dest; subst; disc_rule_conds.
+          eapply obj_same_id_in_system_same in H23; eauto; subst.
+          left; red; repeat (simpl; mred).
+        * apply InMP_deqMsgs in H6.
+          specialize (H3 H6).
+          destruct (eq_nat_dec (obj_idx obj) (obj_idx pobj)).
+          { eapply obj_same_id_in_system_same in e; eauto; subst.
+            left; red; repeat (simpl; mred).
+          }
+          { destruct H3.
+            { left; red; repeat (simpl; mred). }
+            { rewrite <-H29 in H31.
+              dest; right; split.
+              { red in H3; red; mred.
+                destruct (orqs@[obj_idx pobj]) eqn:Horq; simpl in *; auto.
+                destruct (o@[downRq]) eqn:Hrqid; simpl in *; auto.
+                intros; specialize (H3 _ _ H32 H33 H34).
+                disc_rule_conds.
+                assert (obj_idx upCObj <> obj_idx cobj)
+                  by (intro Hx; rewrite Hx in *; disc_rule_conds; auto).
+                solve_q; assumption.
+              }
+              { apply FirstMP_enqMP.
+                apply FirstMP_deqMsgs; [|eassumption].
+                solve_midx_disj.
+              }
+            }
+          }
+            
+      + apply InMP_enqMP_or in H27; destruct H27;
+          [dest; subst; solve_midx_false|].
+        apply InMP_deqMsgs in H22.
+        specialize (H3 H22).
+        destruct (eq_nat_dec (obj_idx obj) (obj_idx pobj)).
+        * eapply obj_same_id_in_system_same in e; eauto; subst.
+          left; red; repeat (simpl; mred).
+        * destruct H3.
+          { left; red; repeat (simpl; mred). }
+          { rewrite <-H29 in H7.
+            dest; right; split.
+            { red in H3; red; mred.
+              destruct (orqs@[obj_idx pobj]) eqn:Horq; simpl in *; auto.
+              destruct (o@[downRq]) eqn:Hrqid; simpl in *; auto.
+              intros; specialize (H3 _ _ H30 H31 H32).
+              disc_rule_conds.
+              solve_q; assumption.
+            }
+            { apply FirstMP_enqMP.
+              apply FirstMP_deqMsgs; [|eassumption].
+              solve_midx_disj.
+            }
+          }
+
+    - disc_rule_conds.
+      apply InMP_enqMsgs_or in H28; destruct H28.
+      1:{ exfalso.
+          rewrite Forall_forall in H27; specialize (H27 _ H5).
+          simpl in H27; rewrite H26 in H27; discriminate.
+      }
+
+      destruct (eq_nat_dec (obj_idx obj) (obj_idx pobj)).
+      + apply InMP_deqMP in H5.
+        specialize (H3 H5).
+        eapply obj_same_id_in_system_same in e; eauto; subst.
+        right; split.
+        * destruct (in_dec eq_nat_dec down (idsOf routs)).
+          { red; repeat (simpl; mred).
+            intros; solve_q.
+            destruct H19.
+            apply in_map_iff in i; destruct i as [[down' rqdm] ?]; dest.
+            simpl in *; subst.
+            erewrite findQ_In_NoDup_enqMsgs; try eassumption.
+            rewrite Forall_forall in H27; specialize (H27 _ H36); simpl in H27.
+            rewrite filter_app; simpl.
+            rewrite H27; simpl.
+            destruct (filter _ _); discriminate.
+          }
+          { red; repeat (simpl; mred).
+            intros; disc_rule_conds.
+            elim n; clear n.
+            eapply RqRsDownMatch_rs_rq in H20; [|eassumption].
+            destruct H20 as [cidx [rdown ?]]; dest.
+            disc_rule_conds.
+          }
+        * apply FirstMP_enqMsgs.
+          apply FirstMP_deqMP.
+          { apply parentIdxOf_not_eq in H24; [|apply Hrrs].
+            solve_midx_neq.
+          }
+          { (* [rqsQ down msgs = nil] since [porq@[downRq] = None].
+             * Then we need to prove:
+             * [InMP down rsdm msgs -> rqsQ down msgs = nil -> FirstMP down rsdm msgs]
+             *)
+            admit.
+          }
+
+      + destruct (eq_nat_dec (obj_idx obj) (obj_idx cobj)).
+        * eapply obj_same_id_in_system_same in e; eauto; subst.
+          disc_rule_conds.
+          exfalso.
+          (* H5 is false. *)
+          admit.
+        * apply InMP_deqMP in H5.
+          specialize (H3 H5).
+          destruct H3; [left; red; mred|].
+          dest; right; split.
+          { red in H3; red; mred.
+            destruct (orqs@[obj_idx pobj]) eqn:Horq; simpl in *; auto.
+            destruct (o@[downRq]) eqn:Hrqid; simpl in *; auto.
+            intros; specialize (H3 _ _ H30 H32 H33).
+            disc_rule_conds.
+            assert (Some (obj_idx pobj) <> Some (obj_idx obj)) by congruence.
+            solve_q; assumption.
+          }
+          { apply FirstMP_enqMsgs.
+            apply FirstMP_deqMP; [|assumption].
+            solve_midx_neq.
+          }
+    
+  Admitted.
+  
+  Lemma noRqRsDown_InvStep:
+    InvStep sys step_m NoRqRsDown.
+  Proof.
+    destruct Hrrs as [? [? ?]]; red; intros.
+    inv H4.
+    - assumption.
+    - apply noRqRsDown_step_ext_in; auto.
+    - apply noRqRsDown_step_ext_out; auto.
+    - eapply noRqRsDown_step_int; eauto.
+      econstructor; eauto.
+  Qed.
+
+End RqRsDown.
+
 Close Scope list.
 Close Scope fmap.
+
